revive header_encrypt/header_decrypt correctness

src/QUIC.Spec.Header.fst
@@ -1,13 +1,420 @@
 module QUIC.Spec.Header
 
 module PN = QUIC.Spec.PacketNumber
-module Public = QUIC.Spec.Header.Public
-module LP = LowParse.Spec.Combinators
 module Secret = QUIC.Secret.Int
 module BF = LowParse.BitFields
 module U8 = FStar.UInt8
 module Seq = QUIC.Secret.Seq
 module U64 = FStar.UInt64
+module Parse = QUIC.Spec.Header.Parse
+
+module AEAD = Spec.Agile.AEAD
+module Cipher = Spec.Agile.Cipher
+module Lemmas = QUIC.Spec.Lemmas
+
+let block_of_sample
+  (a: Cipher.cipher_alg)
+  (k: Cipher.key a)
+  (sample: lbytes 16)
+: GTot (lbytes 16) =
+  let open FStar.Mul in
+  let ctr, iv = match a with
+    | Cipher.CHACHA20 ->
+        let ctr_bytes, iv = Seq.split sample 4 in
+        let iv = Seq.seq_hide #Secret.U8 iv in
+        FStar.Endianness.lemma_le_to_n_is_bounded ctr_bytes;
+        assert_norm (pow2 (8 * 4) = pow2 32);
+        FStar.Endianness.le_to_n ctr_bytes, iv
+    | _ ->
+        let iv, ctr_bytes = Seq.split sample 12 in
+        let iv = Seq.seq_hide #Secret.U8 iv in
+        FStar.Endianness.lemma_be_to_n_is_bounded ctr_bytes;
+        assert_norm (pow2 (8 * 4) = pow2 32);
+        FStar.Endianness.be_to_n ctr_bytes, iv
+  in
+  Seq.seq_reveal (Seq.slice (Cipher.ctr_block a k iv ctr) 0 16)
+
+(*
+Decryption of packet number
+packet[pn_offset..pn_offset+4] ^= pn_mask &
+  match pn_len with
+  | 0 -> mask & 0xFF000000
+  | 1 -> mask & 0xFFFF0000
+  | 2 -> mask & 0xFFFFFF00
+  | 3 -> mask & 0xFFFFFFFF
+*)
+let pn_sizemask' (pn_len: nat { pn_len < 4 }) : Tot (lbytes 4) =
+  let open FStar.Endianness in
+  FStar.Math.Lemmas.pow2_lt_compat 32 (24 - (8 `op_Multiply` pn_len));
+  FStar.Endianness.n_to_be 4 (pow2 32 - pow2 (24 - (8 `op_Multiply` pn_len)))
+
+let pn_sizemask (pn_len: nat { pn_len < 4 }) : Tot (lbytes (pn_len + 1)) =
+  Seq.slice (pn_sizemask' pn_len) 0 (pn_len + 1)
+
+let header_encrypt
+  a hpk h c
+=
+  assert_norm(max_cipher_length < pow2 62);
+  let r = Parse.format_header h `Seq.append` c in
+  if is_retry h
+  then
+    r
+  else
+    let pn_offset = Parse.pn_offset h in
+    let pn_len = Secret.v (pn_length h) - 1 in
+    let sample = Seq.slice c (3-pn_len) (19-pn_len) in
+    let mask = block_of_sample (AEAD.cipher_alg_of_supported_alg a) hpk sample in
+    let pnmask = Lemmas.and_inplace (Seq.slice mask 1 (pn_len + 2)) (pn_sizemask pn_len) 0 in
+    let f = Seq.index r 0 in
+    let protected_bits = if MShort? h then 5 else 4 in
+    let f' = BF.set_bitfield (U8.v f) 0 protected_bits (BF.get_bitfield (U8.v f `FStar.UInt.logxor` U8.v (Seq.index mask 0)) 0 protected_bits) in
+    let r = Lemmas.xor_inplace r pnmask pn_offset in
+    let r = Seq.cons (U8.uint_to_t f') (Seq.slice r 1 (Seq.length r)) in
+    r
+
+#push-options "--z3rlimit 128"
+
+#restart-solver
+
+let header_encrypt_post
+  (a:ea)
+  (hpk: Cipher.key (AEAD.cipher_alg_of_supported_alg a))
+  (h: header)
+  (c: cbytes' (is_retry h))
+  (cid_len: nat { cid_len <= 20 /\ (MShort? h ==> cid_len == dcid_len h) })
+: Lemma (
+    let x = Parse.format_header h in
+    let y = x `Seq.append` c in
+    let z = header_encrypt a hpk h c in
+    Parse.header_len h + Seq.length c == Seq.length z /\
+    Seq.slice z (Parse.header_len h) (Seq.length z) `Seq.equal` c /\
+    MShort? h == (BF.get_bitfield (U8.v (Seq.index z 0)) 7 8 = 0) /\
+    is_retry h == (not (MShort? h) && BF.get_bitfield (U8.v (Seq.index z 0)) 4 6 = 3) /\ (
+    if is_retry h
+    then z == y
+    else Parse.putative_pn_offset cid_len z == Some (Parse.pn_offset h)
+  ))
+= Parse.format_header_is_short h;
+  Parse.format_header_is_retry h;
+  if is_retry h
+  then ()
+  else begin
+    Parse.format_header_pn_length h;
+    let x = Parse.format_header h in
+    let y = x `Seq.append` c in
+    let pn_offset = Parse.pn_offset h in
+    let pn_len = Secret.v (pn_length h) - 1 in
+    let sample = Seq.slice c (3-pn_len) (19-pn_len) in
+    let mask = block_of_sample (AEAD.cipher_alg_of_supported_alg a) hpk sample in
+    let pnmask = Lemmas.and_inplace (Seq.slice mask 1 (pn_len + 2)) (pn_sizemask pn_len) 0 in
+    let f = Seq.index y 0 in
+    let protected_bits = if MShort? h then 5 else 4 in
+    let bf = BF.get_bitfield (U8.v f `FStar.UInt.logxor` U8.v (Seq.index mask 0)) 0 protected_bits in
+    let f' = BF.set_bitfield (U8.v f) 0 protected_bits bf in
+    let r = Lemmas.xor_inplace y pnmask pn_offset in
+    let z = header_encrypt a hpk h c in
+    assert (z == Seq.cons (U8.uint_to_t f') (Seq.slice r 1 (Seq.length r)));
+    Lemmas.pointwise_op_slice_other U8.logxor y pnmask pn_offset 0 1;
+    Lemmas.pointwise_op_slice_other U8.logxor y pnmask pn_offset 1 pn_offset;
+    assert (pn_offset > 0);
+    Lemmas.pointwise_op_slice_other U8.logxor y pnmask pn_offset (Parse.header_len h) (Seq.length y);
+    assert (Seq.slice z (Parse.header_len h) (Seq.length z) `Seq.equal` Seq.slice y (Parse.header_len h) (Seq.length y));
+    assert (U8.uint_to_t f' == Seq.index (Seq.slice z 0 1) 0);
+    BF.get_bitfield_set_bitfield_other (U8.v f) 0 protected_bits bf 7 8;
+    BF.get_bitfield_set_bitfield_other (U8.v f) 0 protected_bits bf protected_bits 8;
+    if MLong? h
+    then BF.get_bitfield_set_bitfield_other (U8.v f) 0 protected_bits bf 4 6;
+    Parse.putative_pn_offset_correct h cid_len;
+    Parse.putative_pn_offset_frame cid_len x y;
+    Parse.putative_pn_offset_frame cid_len y z;
+    ()
+  end
+
+#pop-options
+
+noextract
+type header_decrypt_aux_t = {
+  is_short: bool;
+  is_retry: (is_retry: bool { is_retry ==> ~ (is_short) });
+  packet: packet;
+  pn_offset: (if is_retry then unit else nat);
+  pn_len: (if is_retry then unit else (pn_len: nat {pn_len < 4 /\ pn_offset + pn_len + 1 <= Seq.length packet}));
+}
+
+let header_decrypt_aux
+  (a:ea)
+  (hpk: Cipher.key (AEAD.cipher_alg_of_supported_alg a))
+  (cid_len: nat { cid_len <= 20 })
+  (packet: packet)
+: GTot (option header_decrypt_aux_t)
+= let open FStar.Math.Lemmas in
+  if Seq.length packet = 0
+  then None
+  else
+    let f = Seq.index packet 0 in
+    let is_short = (BF.get_bitfield (U8.v f) 7 8 = 0) in
+    let is_retry = not is_short && BF.get_bitfield (U8.v f) 4 6 = 3 in
+    if is_retry
+    then
+      Some ({
+        is_short = is_short;
+        is_retry = is_retry;
+        packet = packet;
+        pn_offset = ();
+        pn_len = ();
+      })
+    else
+      match Parse.putative_pn_offset cid_len packet with
+      | None -> None
+      | Some pn_offset ->
+        let sample_offset = pn_offset + 4 in
+        if sample_offset + 16 > Seq.length packet
+        then None
+        else begin
+          let sample = Seq.slice packet sample_offset (sample_offset+16) in
+          let mask = block_of_sample (AEAD.cipher_alg_of_supported_alg a) hpk sample in
+          (* mask the least significant bits of the first byte *)
+          let protected_bits = if is_short then 5 else 4 in
+          let f' = BF.set_bitfield (U8.v f) 0 protected_bits (BF.get_bitfield (U8.v f `FStar.UInt.logxor` U8.v (Seq.index mask 0)) 0 protected_bits) in
+          let packet' = Seq.cons (U8.uint_to_t f') (Seq.slice packet 1 (Seq.length packet)) in
+          (* now the packet number length is available, so mask the packet number *)
+          let pn_len = BF.get_bitfield f' 0 2 in
+          let pnmask = Lemmas.and_inplace (Seq.slice mask 1 (pn_len + 2)) (pn_sizemask pn_len) 0 in
+          let packet'' = Lemmas.xor_inplace packet' pnmask pn_offset in
+          Some ({
+            is_short = is_short;
+            is_retry = is_retry;
+            packet = packet'';
+            pn_offset = pn_offset;
+            pn_len = pn_len;
+          })
+        end
+
+#push-options "--z3rlimit 32 --max_fuel 1"
+
+let header_decrypt_aux_post
+  (a:ea)
+  (hpk: Cipher.key (AEAD.cipher_alg_of_supported_alg a))
+  (cid_len: nat { cid_len <= 20 })
+  (packet: packet)
+: Lemma
+  (requires (Some? (header_decrypt_aux a hpk cid_len packet)))
+  (ensures (
+    let Some r = header_decrypt_aux a hpk cid_len packet in
+    Seq.length r.packet == Seq.length packet /\
+    Seq.length packet > 0 /\ (
+    let f' = Seq.index r.packet 0 in
+    r.is_short == (BF.get_bitfield (U8.v f') 7 8 = 0) /\
+    r.is_retry == (not r.is_short && (BF.get_bitfield (U8.v f') 4 6 = 3)) /\ (
+    if r.is_retry
+    then r.packet == packet
+    else
+      Some? (Parse.putative_pn_offset cid_len packet) /\
+      Parse.putative_pn_offset cid_len r.packet == Parse.putative_pn_offset cid_len packet /\ (
+      let Some pn_offset = Parse.putative_pn_offset cid_len packet in
+      r.pn_len == BF.get_bitfield (U8.v f') 0 2 /\
+      Seq.slice r.packet (r.pn_offset + r.pn_len + 1) (Seq.length r.packet) `Seq.equal` Seq.slice packet (r.pn_offset + r.pn_len + 1) (Seq.length packet) /\
+      True
+  )))))
+= let Some r = header_decrypt_aux a hpk cid_len packet in
+  let f = Seq.index packet 0 in
+  let is_short = (BF.get_bitfield (U8.v f) 7 8 = 0) in
+  let is_retry = not is_short && BF.get_bitfield (U8.v f) 4 6 = 3 in
+  if is_retry
+  then ()
+  else begin
+    let Some pn_offset = Parse.putative_pn_offset cid_len packet in
+    let sample_offset = pn_offset + 4 in
+    let sample = Seq.slice packet sample_offset (sample_offset+16) in
+    let mask = block_of_sample (AEAD.cipher_alg_of_supported_alg a) hpk sample in
+    (* mask the least significant bits of the first byte *)
+    let protected_bits = if is_short then 5 else 4 in
+    let bf = BF.get_bitfield (U8.v f `FStar.UInt.logxor` U8.v (Seq.index mask 0)) 0 protected_bits in
+    let f' = BF.set_bitfield (U8.v f) 0 protected_bits bf in
+    let packet' = Seq.cons (U8.uint_to_t f') (Seq.slice packet 1 (Seq.length packet)) in
+    (* now the packet number length is available, so mask the packet number *)
+    let pn_len = BF.get_bitfield f' 0 2 in
+    let pnmask = Lemmas.and_inplace (Seq.slice mask 1 (pn_len + 2)) (pn_sizemask pn_len) 0 in
+    assert (r.packet == Lemmas.xor_inplace packet' pnmask pn_offset);
+    Lemmas.pointwise_op_slice_other U8.logxor packet' pnmask pn_offset 0 1;
+    Lemmas.pointwise_op_slice_other U8.logxor packet' pnmask pn_offset 1 pn_offset;
+    Lemmas.pointwise_op_slice_other U8.logxor packet' pnmask pn_offset (pn_offset + pn_len + 1) (Seq.length packet);
+    BF.get_bitfield_set_bitfield_other (U8.v f) 0 protected_bits bf protected_bits 8;
+    BF.get_bitfield_set_bitfield_other (U8.v f) 0 protected_bits bf 7 8;
+    assert (Seq.index r.packet 0 == Seq.index (Seq.slice packet' 0 1) 0);
+    Parse.putative_pn_offset_frame cid_len packet r.packet;
+    if not is_short
+    then BF.get_bitfield_set_bitfield_other (U8.v f) 0 protected_bits bf 4 6;
+    assert (Parse.putative_pn_offset cid_len r.packet == Parse.putative_pn_offset cid_len packet);
+    ()
+  end
+
+#pop-options
+
+#push-options "--z3rlimit 64 --max_fuel 1"
+
+let header_decrypt_aux_post_parse
+  (a:ea)
+  (hpk: Cipher.key (AEAD.cipher_alg_of_supported_alg a))
+  (cid_len: nat { cid_len <= 20 })
+  (last: nat { last + 1 < pow2 62 })
+  (packet: packet)
+: Lemma
+  (requires (match header_decrypt_aux a hpk cid_len packet with
+    | Some r ->
+      Parse.H_Success? (Parse.parse_header cid_len last r.packet)
+    | _ -> False
+  ))
+  (ensures (
+    let Some r = header_decrypt_aux a hpk cid_len packet in
+    let Parse.H_Success h rem' = Parse.parse_header cid_len last r.packet in
+    Parse.header_len h <= Seq.length packet /\
+    Seq.length r.packet == Seq.length packet /\
+    Seq.length packet > 0 /\ (
+    r.is_short == MShort? h /\
+    r.is_retry == is_retry h /\
+    rem' `Seq.equal` Seq.slice packet (Parse.header_len h) (Seq.length packet) /\ (
+    if r.is_retry
+    then r.packet == packet
+    else
+      Some? (Parse.putative_pn_offset cid_len packet) /\ (
+      let Some pn_offset = Parse.putative_pn_offset cid_len packet in
+      pn_offset == Parse.pn_offset h /\
+      r.pn_len == Secret.v (pn_length h) - 1 /\
+      r.pn_offset + r.pn_len + 1 == Parse.header_len h /\
+      True
+  )))))
+= header_decrypt_aux_post a hpk cid_len packet;
+  let Some r = header_decrypt_aux a hpk cid_len packet in
+  let Parse.H_Success h rem' = Parse.parse_header cid_len last r.packet in
+  Parse.lemma_header_parsing_post cid_len last r.packet;
+  Parse.format_header_is_short h;
+  Parse.format_header_is_retry h;
+  assert (r.is_short == MShort? h);
+  assert (r.is_retry == is_retry h);
+  if r.is_retry
+  then
+    ()
+  else begin
+    Parse.format_header_pn_length h;
+    let Some pn_offset = Parse.putative_pn_offset cid_len packet in
+    Parse.putative_pn_offset_correct h cid_len;
+    Parse.putative_pn_offset_frame cid_len (Parse.format_header h) r.packet
+  end
+
+#pop-options
+
+#push-options "--z3rlimit 128"
+
+let header_decrypt
+  a hpk cid_len last packet
+=
+  let open FStar.Math.Lemmas in
+  if Seq.length packet = 0
+  then H_Failure
+  else
+    match header_decrypt_aux a hpk cid_len packet with
+    | None -> H_Failure
+    | Some r ->
+      let packet'' = r.packet in
+      begin match Parse.parse_header cid_len last packet'' with
+      | Parse.H_Failure -> H_Failure
+      | Parse.H_Success h rem' ->
+        header_decrypt_aux_post_parse a hpk cid_len last packet;
+        if is_retry h
+        then
+          H_Success h Seq.empty rem'
+        else if has_payload_length h && Seq.length rem' < Secret.v (payload_length h)
+        then H_Failure
+        else
+          let clen = if has_payload_length h then Secret.v (payload_length h) else Seq.length rem' in
+          if 19 <= clen && clen < max_cipher_length
+          then
+            let c : cbytes = Seq.slice rem' 0 clen in
+            let rem = Seq.slice rem' clen (Seq.length rem') in
+            H_Success h c rem
+          else
+            H_Failure
+      end
+
+let lemma_header_encryption_correct_aux
+  (a:ea)
+  (k: Cipher.key (AEAD.cipher_alg_of_supported_alg a))
+  (h:header)
+  (cid_len: nat { cid_len <= 20 /\ (MShort? h ==> cid_len == dcid_len h) })
+  (c: cbytes' (is_retry h)) // { has_payload_length h ==> U64.v (payload_length h) == Seq.length c } ->
+: Lemma
+  (let r' = header_decrypt_aux a k cid_len (header_encrypt a k h c) in
+   Some? r' /\ (
+   let Some r = r' in
+   r.packet `Seq.equal` (Parse.format_header h `Seq.append` c) /\
+   r.is_short == MShort? h /\
+   r.is_retry == is_retry h /\
+   ((~ (is_retry h)) ==> ((r.pn_offset <: nat) == Parse.pn_offset h /\ r.pn_len == Secret.v (pn_length h) - 1))
+  ))
+= header_encrypt_post a k h c cid_len;
+  header_decrypt_aux_post a k cid_len (header_encrypt a k h c);
+  if is_retry h
+  then
+    ()
+  else begin
+    let format = Parse.format_header h `Seq.append` c in
+    let packet = header_encrypt a k h c in
+    let Some r = header_decrypt_aux a k cid_len packet in
+    Parse.putative_pn_offset_correct h cid_len;
+    let pn_offset = Parse.pn_offset h in
+    let pn_len = Secret.v (pn_length h) - 1 in
+    let sample = Seq.slice c (3-pn_len) (19-pn_len) in
+    assert (sample `Seq.equal` Seq.slice packet (pn_offset + 4) (pn_offset + 20));
+    assert ((r.pn_offset <: nat) == pn_offset);
+    let mask = block_of_sample (AEAD.cipher_alg_of_supported_alg a) k sample in
+    let protected_bits = if MShort? h then 5 else 4 in
+    assert (protected_bits == (if r.is_short then 5 else 4));
+    let f = Seq.index format 0 in
+    let pb_value = BF.get_bitfield (U8.v f `FStar.UInt.logxor` U8.v (Seq.index mask 0)) 0 protected_bits in
+    let f0 = BF.set_bitfield (U8.v f) 0 protected_bits pb_value in
+    assert (U8.uint_to_t f0 == Seq.index packet 0);
+    let pb_value' = BF.get_bitfield (f0 `FStar.UInt.logxor` U8.v (Seq.index mask 0)) 0 protected_bits in
+    let f1 = BF.set_bitfield f0 0 protected_bits pb_value' in
+    let packet1 = Seq.cons (U8.uint_to_t f1) (Seq.slice packet 1 (Seq.length packet)) in
+    let pnmask' = Lemmas.and_inplace (Seq.slice mask 1 (r.pn_len + 2)) (pn_sizemask r.pn_len) 0 in
+    assert (r.packet == Lemmas.xor_inplace packet1 pnmask' pn_offset);
+    Lemmas.pointwise_op_slice_other U8.logxor packet1 pnmask' pn_offset 0 1;
+    assert (Seq.index r.packet 0 == Seq.index (Seq.slice r.packet 0 1) 0);
+    assert (Seq.index r.packet 0 == U8.uint_to_t f1);
+    BF.get_bitfield_logxor (U8.v f) (U8.v (Seq.index mask 0)) 0 protected_bits;
+    BF.get_bitfield_set_bitfield_same (U8.v f) 0 protected_bits pb_value;
+    BF.get_bitfield_logxor (f0) (U8.v (Seq.index mask 0)) 0 protected_bits;
+    BF.get_bitfield_set_bitfield_same (f0) 0 protected_bits pb_value';
+    FStar.UInt.logxor_inv (BF.get_bitfield (U8.v f) 0 protected_bits) (BF.get_bitfield (U8.v (Seq.index mask 0)) 0 protected_bits);
+    assert (BF.get_bitfield (U8.v f) 0 protected_bits == BF.get_bitfield f1 0 protected_bits);
+    BF.get_bitfield_set_bitfield_other (U8.v f) 0 protected_bits pb_value protected_bits 8;
+    BF.get_bitfield_set_bitfield_other (f0) 0 protected_bits pb_value' protected_bits 8;
+    BF.get_bitfield_partition_2 protected_bits (U8.v f) f1;
+    assert (f == U8.uint_to_t f1);
+    Parse.format_header_pn_length h;
+    assert ((r.pn_len <: nat) == pn_len);
+    assert (pnmask' == Lemmas.and_inplace (Seq.slice mask 1 (pn_len + 2)) (pn_sizemask pn_len) 0);
+    Lemmas.xor_inplace_involutive format pnmask' pn_offset;
+    let packet0 = Lemmas.xor_inplace format pnmask' pn_offset in
+    Lemmas.pointwise_op_slice_other U8.logxor format pnmask' pn_offset 0 1;
+    assert (Seq.index packet0 0 == Seq.index (Seq.slice format 0 1) 0);
+    assert (packet == Seq.cons (U8.uint_to_t f0) (Seq.slice packet0 1 (Seq.length packet0)));
+    assert (packet1 `Seq.equal` Seq.cons (U8.uint_to_t f1) (Seq.slice packet0 1 (Seq.length packet0)));
+    assert (packet1 `Seq.equal` packet0);
+    assert (r.packet `Seq.equal` format);
+    ()
+  end
+
+#pop-options
+
+let lemma_header_encryption_correct
+  a k h cid_len last c
+=
+  lemma_header_encryption_correct_aux a k h cid_len c;
+  Parse.lemma_header_parsing_correct h c cid_len last
+
+
 
 (*
 let parse_header
@@ -62,49 +469,6 @@ let lemma_header_parsing_safe
     Seq.lemma_split b2 consumed
 
 #pop-options
-
-let block_of_sample
-  (a: Cipher.cipher_alg)
-  (k: Cipher.key a)
-  (sample: lbytes 16)
-: GTot (lbytes 16) =
-  let open FStar.Mul in
-  let ctr, iv = match a with
-    | Cipher.CHACHA20 ->
-        let ctr_bytes, iv = Seq.split sample 4 in
-        let iv = Seq.seq_hide #Secret.U8 iv in
-        FStar.Endianness.lemma_le_to_n_is_bounded ctr_bytes;
-        assert_norm (pow2 (8 * 4) = pow2 32);
-        FStar.Endianness.le_to_n ctr_bytes, iv
-    | _ ->
-        let iv, ctr_bytes = Seq.split sample 12 in
-        let iv = Seq.seq_hide #Secret.U8 iv in
-        FStar.Endianness.lemma_be_to_n_is_bounded ctr_bytes;
-        assert_norm (pow2 (8 * 4) = pow2 32);
-        FStar.Endianness.be_to_n ctr_bytes, iv
-  in
-  Seq.seq_reveal (Seq.slice (Cipher.ctr_block a k iv ctr) 0 16)
-
-(*
-Decryption of packet number
-packet[pn_offset..pn_offset+4] ^= pn_mask &
-  match pn_len with
-  | 0 -> mask & 0xFF000000
-  | 1 -> mask & 0xFFFF0000
-  | 2 -> mask & 0xFFFFFF00
-  | 3 -> mask & 0xFFFFFFFF
-*)
-inline_for_extraction
-let pn_sizemask' (pn_len: nat { pn_len < 4 }) : lbytes 4 =
-  let open FStar.Endianness in
-  FStar.Math.Lemmas.pow2_lt_compat 32 (24 - (8 `op_Multiply` pn_len));
-  FStar.Endianness.n_to_be 4 (pow2 32 - pow2 (24 - (8 `op_Multiply` pn_len)))
-
-inline_for_extraction
-let pn_sizemask (pn_len: nat { pn_len < 4 }) : lbytes (pn_len + 1) =
-  Seq.slice (pn_sizemask' pn_len) 0 (pn_len + 1)
-
-module Lemmas = QUIC.Spec.Lemmas
 
 #push-options "--z3rlimit 16"
 
@@ -188,29 +552,6 @@ let pn_offset_prop
   PN.parse_packet_number_kind'_correct last pn_len;
   let (| _, pn |) = synth_header_recip cid_len last h in
   LP.serialize_length #(PN.parse_packet_number_kind' pn_len) #_ #(PN.parse_packet_number last pn_len <: LP.bare_parser (PN.packet_number_t' last pn_len)) (PN.serialize_packet_number last pn_len <: LP.bare_serializer (PN.packet_number_t' last pn_len)) pn
-
-let header_encrypt
-  a hpk h c
-=
-  assert_norm(max_cipher_length < pow2 62);
-  let r = format_header h `Seq.append` c in
-  let _ = format_header_bound h in
-  if is_retry h
-  then
-    r
-  else
-    let pn_offset = pn_offset h in
-    let _ = pn_offset_prop h in
-    let pn_len = Secret.v (pn_length h) - 1 in
-    let sample = Seq.slice c (3-pn_len) (19-pn_len) in
-    let mask = block_of_sample (AEAD.cipher_alg_of_supported_alg a) hpk sample in
-    let pnmask = Lemmas.and_inplace (Seq.slice mask 1 (pn_len + 2)) (pn_sizemask pn_len) 0 in
-    let f = Seq.index r 0 in
-    let protected_bits = if MShort? h then 5 else 4 in
-    let f' = BF.set_bitfield (U8.v f) 0 protected_bits (BF.get_bitfield (U8.v f `FStar.UInt.logxor` U8.v (Seq.index mask 0)) 0 protected_bits) in
-    let r = Lemmas.xor_inplace r pnmask pn_offset in
-    let r = Seq.cons (U8.uint_to_t f') (Seq.slice r 1 (Seq.length r)) in
-    r
 
 assume
 val header_decrypt_only_correct
@@ -975,7 +1316,7 @@ val pn_offset'
     let s = serialize (serialize_header short_dcid_len last) h in
     0 < n /\
     n + U32.v (pn_length h) == Seq.length s /\
-    S.slice s n (S.length s) `S.equal` serialize (serialize_packet_number last (pn_length h)) (packet_number h)
+    Seq.slice s n (Seq.length s) `Seq.equal` serialize (serialize_packet_number last (pn_length h)) (packet_number h)
   ))
 
 #push-options "--z3rlimit 1024 --query_stats --max_fuel 4 --initial_fuel 4"
@@ -994,7 +1335,7 @@ let pn_offset'
     assert_norm (bitsum'_key_of_t first_byte (first_byte_of_header short_dcid_len last (MShort spin key_phase dcid packet_number_length packet_number)) == (| Short, (| (), (| (), (| packet_number_length, () |) |) |) |) ) ;
     serialize_nondep_then_eq (serialize_weaken (strong_parser_kind 0 20 None) (serialize_flbytes (U32.v short_dcid_len))) (serialize_packet_number last packet_number_length) (dcid, packet_number);
     serialize_length (serialize_packet_number last packet_number_length) packet_number;
-    1 + S.length (serialize (serialize_weaken (strong_parser_kind 0 20 None) (serialize_flbytes (U32.v short_dcid_len))) dcid)
+    1 + Seq.length (serialize (serialize_weaken (strong_parser_kind 0 20 None) (serialize_flbytes (U32.v short_dcid_len))) dcid)
   | MLong version dcid scid spec ->
     begin match spec with
     | MInitial token payload_length packet_number_length packet_number ->
@@ -1005,7 +1346,7 @@ let pn_offset'
       serialize_nondep_then_eq (serialize_bounded_vlgenbytes 0 token_max_len (serialize_bounded_varint 0 token_max_len)) (serialize_payload_length_pn last packet_number_length) (token, (plpnl, packet_number));
       serialize_nondep_then_eq (serialize_varint `serialize_filter` payload_and_pn_length_prop packet_number_length) (serialize_packet_number last packet_number_length) (plpnl, packet_number);
       serialize_length (serialize_packet_number last packet_number_length) packet_number;
-      1 + S.length (serialize serialize_common_long (version, (dcid, scid))) + S.length (serialize (serialize_bounded_vlgenbytes 0 token_max_len (serialize_bounded_varint 0 token_max_len)) token) + S.length (serialize (serialize_varint `serialize_filter` payload_and_pn_length_prop packet_number_length) plpnl)
+      1 + Seq.length (serialize serialize_common_long (version, (dcid, scid))) + Seq.length (serialize (serialize_bounded_vlgenbytes 0 token_max_len (serialize_bounded_varint 0 token_max_len)) token) + Seq.length (serialize (serialize_varint `serialize_filter` payload_and_pn_length_prop packet_number_length) plpnl)
     | MHandshake payload_length packet_number_length packet_number ->
       assert_norm (first_byte_of_header short_dcid_len last (MLong version dcid scid (MHandshake payload_length packet_number_length packet_number)) == (| Long, (| (), (| Handshake, (| (), (| packet_number_length, () |) |) |) |) |) );
       assert_norm (bitsum'_key_of_t first_byte (first_byte_of_header short_dcid_len last (MLong version dcid scid (MHandshake payload_length packet_number_length packet_number))) == (| Long, (| (), (| Handshake, (| (), (| packet_number_length, () |) |) |) |) |) );
@@ -1013,7 +1354,7 @@ let pn_offset'
       serialize_nondep_then_eq serialize_common_long (serialize_payload_length_pn last packet_number_length) ((version, (dcid, scid)), (plpnl, packet_number));
       serialize_nondep_then_eq (serialize_varint `serialize_filter` payload_and_pn_length_prop packet_number_length) (serialize_packet_number last packet_number_length) (plpnl, packet_number);
       serialize_length (serialize_packet_number last packet_number_length) packet_number;
-      1 + S.length (serialize serialize_common_long (version, (dcid, scid))) + S.length (serialize (serialize_varint `serialize_filter` payload_and_pn_length_prop packet_number_length) plpnl)
+      1 + Seq.length (serialize serialize_common_long (version, (dcid, scid))) + Seq.length (serialize (serialize_varint `serialize_filter` payload_and_pn_length_prop packet_number_length) plpnl)
     | MZeroRTT payload_length packet_number_length packet_number ->
       assert_norm (first_byte_of_header short_dcid_len last (MLong version dcid scid (MZeroRTT payload_length packet_number_length packet_number)) == (| Long, (| (), (| ZeroRTT, (| (), (| packet_number_length, () |) |) |) |) |) );
       assert_norm (bitsum'_key_of_t first_byte (first_byte_of_header short_dcid_len last (MLong version dcid scid (MZeroRTT payload_length packet_number_length packet_number))) == (| Long, (| (), (| ZeroRTT, (| (), (| packet_number_length, () |) |) |) |) |) );
@@ -1021,7 +1362,7 @@ let pn_offset'
       serialize_nondep_then_eq serialize_common_long (serialize_payload_length_pn last packet_number_length) ((version, (dcid, scid)), (plpnl, packet_number));
       serialize_nondep_then_eq (serialize_varint `serialize_filter` payload_and_pn_length_prop packet_number_length) (serialize_packet_number last packet_number_length) (plpnl, packet_number);
       serialize_length (serialize_packet_number last packet_number_length) packet_number;
-      1 + S.length (serialize serialize_common_long (version, (dcid, scid))) + S.length (serialize (serialize_varint `serialize_filter` payload_and_pn_length_prop packet_number_length) plpnl)
+      1 + Seq.length (serialize serialize_common_long (version, (dcid, scid))) + Seq.length (serialize (serialize_varint `serialize_filter` payload_and_pn_length_prop packet_number_length) plpnl)
     end
 
 #pop-options
@@ -1135,8 +1476,8 @@ let putative_pn_offset_frame
 
 val format_header_is_initial: h: header -> Lemma
   ((MLong? h /\ MInitial? (MLong?.spec h))  <==> (
-    BF.get_bitfield (U8.v (S.index (format_header h) 0)) 7 8 == 1 /\
-    BF.get_bitfield (U8.v (S.index (format_header h) 0)) 4 6 == 0
+    BF.get_bitfield (U8.v (Seq.index (format_header h) 0)) 7 8 == 1 /\
+    BF.get_bitfield (U8.v (Seq.index (format_header h) 0)) 4 6 == 0
   ))
 
 #push-options "--z3rlimit 256 --max_fuel 8 --initial_fuel 8 --max_ifuel 8 --initial_ifuel 8"
@@ -1174,10 +1515,10 @@ let putative_pn_offset_correct h cid_len =
   let hd = synth_bitsum'_recip first_byte tg in
   LI.serialize_u8_spec hd;
   parse_serialize serialize_u8 hd;
-  parse_strong_prefix parse_u8 (serialize serialize_u8 hd) (serialize serialize_u8 hd `S.append` serialize (serialize_header_body short_dcid_len last kt) (mk_header_body short_dcid_len last tg h));
+  parse_strong_prefix parse_u8 (serialize serialize_u8 hd) (serialize serialize_u8 hd `Seq.append` serialize (serialize_header_body short_dcid_len last kt) (mk_header_body short_dcid_len last tg h));
   assert (parse parse_u8 x == Some (hd, 1));
-  let x1 = S.slice x 1 (Seq.length x) in
-  assert (x1 `S.equal` serialize (serialize_header_body short_dcid_len last kt) (mk_header_body short_dcid_len last tg h));
+  let x1 = Seq.slice x 1 (Seq.length x) in
+  assert (x1 `Seq.equal` serialize (serialize_header_body short_dcid_len last kt) (mk_header_body short_dcid_len last tg h));
   format_header_is_short h;
   assert (MShort? h <==> uint8.get_bitfield hd 7 8 = 0uy);
   if uint8.get_bitfield hd 7 8 = 0uy
@@ -1193,9 +1534,9 @@ let putative_pn_offset_correct h cid_len =
     assert (serialize (serialize_weaken (strong_parser_kind 0 20 None) (serialize_flbytes cid_len)) (MShort?.dcid h) == serialize (serialize_flbytes cid_len) (MShort?.dcid h));
     parse_serialize (serialize_flbytes cid_len) (MShort?.dcid h);
     parse_strong_prefix (parse_flbytes cid_len) (serialize (serialize_flbytes cid_len) (MShort?.dcid h)) x1;
-    assert (parse (parse_flbytes cid_len) x1 == Some (MShort?.dcid h, S.length (serialize (serialize_weaken (strong_parser_kind 0 20 None) (serialize_flbytes cid_len)) (MShort?.dcid h))));
-    assert (putative_pn_offset cid_len x = Some (1 + S.length (serialize (serialize_weaken (strong_parser_kind 0 20 None) (serialize_flbytes cid_len)) (MShort?.dcid h))));
-    assert_norm (pn_offset' short_dcid_len last (MShort spin key_phase dcid packet_number_length packet_number) == 1 + S.length (serialize (serialize_weaken (strong_parser_kind 0 20 None) (serialize_flbytes (U32.v short_dcid_len))) dcid));
+    assert (parse (parse_flbytes cid_len) x1 == Some (MShort?.dcid h, Seq.length (serialize (serialize_weaken (strong_parser_kind 0 20 None) (serialize_flbytes cid_len)) (MShort?.dcid h))));
+    assert (putative_pn_offset cid_len x = Some (1 + Seq.length (serialize (serialize_weaken (strong_parser_kind 0 20 None) (serialize_flbytes cid_len)) (MShort?.dcid h))));
+    assert_norm (pn_offset' short_dcid_len last (MShort spin key_phase dcid packet_number_length packet_number) == 1 + Seq.length (serialize (serialize_weaken (strong_parser_kind 0 20 None) (serialize_flbytes (U32.v short_dcid_len))) dcid));
     ()
   end else begin
     assert (MLong? h);
@@ -1215,23 +1556,23 @@ let putative_pn_offset_correct h cid_len =
       serialize_nondep_then_eq serialize_common_long (serialize_bounded_vlgenbytes 0 token_max_len (serialize_bounded_varint 0 token_max_len) `serialize_nondep_then` serialize_payload_length_pn last packet_number_length) ((version, (dcid, scid)), (token, (plpnl, packet_number)));
       parse_serialize serialize_common_long (version, (dcid, scid));
       parse_strong_prefix parse_common_long (serialize serialize_common_long (version, (dcid, scid))) x1;
-      let consumed2 = S.length (serialize serialize_common_long (version, (dcid, scid))) in
+      let consumed2 = Seq.length (serialize serialize_common_long (version, (dcid, scid))) in
       assert (parse parse_common_long x1 == Some ((version, (dcid, scid)), consumed2));
-      let x2 = S.slice x1 consumed2 (S.length x1) in
-      assert (x2 `S.equal` serialize (serialize_bounded_vlgenbytes 0 token_max_len (serialize_bounded_varint 0 token_max_len) `serialize_nondep_then` serialize_payload_length_pn last packet_number_length) (token, (plpnl, packet_number)));
+      let x2 = Seq.slice x1 consumed2 (Seq.length x1) in
+      assert (x2 `Seq.equal` serialize (serialize_bounded_vlgenbytes 0 token_max_len (serialize_bounded_varint 0 token_max_len) `serialize_nondep_then` serialize_payload_length_pn last packet_number_length) (token, (plpnl, packet_number)));
       serialize_nondep_then_eq (serialize_bounded_vlgenbytes 0 token_max_len (serialize_bounded_varint 0 token_max_len)) (serialize_payload_length_pn last packet_number_length) (token, (plpnl, packet_number));
       parse_serialize (serialize_bounded_vlgenbytes 0 token_max_len (serialize_bounded_varint 0 token_max_len)) token;
       parse_strong_prefix (parse_bounded_vlgenbytes 0 token_max_len (parse_bounded_varint 0 token_max_len)) (serialize (serialize_bounded_vlgenbytes 0 token_max_len (serialize_bounded_varint 0 token_max_len)) token) x2;
-      let consumed3 = S.length (serialize (serialize_bounded_vlgenbytes 0 token_max_len (serialize_bounded_varint 0 token_max_len)) token) in
+      let consumed3 = Seq.length (serialize (serialize_bounded_vlgenbytes 0 token_max_len (serialize_bounded_varint 0 token_max_len)) token) in
       assert (parse (parse_bounded_vlgenbytes 0 token_max_len (parse_bounded_varint 0 token_max_len)) x2 == Some (token, consumed3));
-      let x3 = S.slice x2 consumed3 (S.length x2) in
-      assert (x3 `S.equal` serialize (serialize_payload_length_pn last packet_number_length) (plpnl, packet_number));
+      let x3 = Seq.slice x2 consumed3 (Seq.length x2) in
+      assert (x3 `Seq.equal` serialize (serialize_payload_length_pn last packet_number_length) (plpnl, packet_number));
       serialize_nondep_then_eq (serialize_varint `serialize_filter` payload_and_pn_length_prop packet_number_length) (serialize_packet_number last packet_number_length) (plpnl, packet_number);
       assert (serialize (serialize_varint `serialize_filter` payload_and_pn_length_prop packet_number_length) plpnl == serialize serialize_varint plpnl);
       parse_serialize serialize_varint plpnl;
       parse_strong_prefix parse_varint (serialize serialize_varint plpnl) x3;
-      let consumed4 = S.length (serialize (serialize_varint `serialize_filter` payload_and_pn_length_prop packet_number_length) plpnl) in
-      assert (consumed4 == S.length (serialize serialize_varint plpnl));
+      let consumed4 = Seq.length (serialize (serialize_varint `serialize_filter` payload_and_pn_length_prop packet_number_length) plpnl) in
+      assert (consumed4 == Seq.length (serialize serialize_varint plpnl));
       assert (parse parse_varint x3 == Some (plpnl, consumed4));
       assert (putative_pn_offset cid_len x = Some (1 + consumed2 + consumed3 + consumed4));
       assert_norm (pn_offset' short_dcid_len last (MLong version dcid scid (MInitial token payload_length packet_number_length packet_number)) == 1 + consumed2 + consumed3 + consumed4)
@@ -1244,18 +1585,18 @@ let putative_pn_offset_correct h cid_len =
         serialize_nondep_then_eq serialize_common_long (serialize_payload_length_pn last packet_number_length) ((version, (dcid, scid)), (plpnl, packet_number));
         parse_serialize serialize_common_long (version, (dcid, scid));
         parse_strong_prefix parse_common_long (serialize serialize_common_long (version, (dcid, scid))) x1;
-        let consumed2 = S.length (serialize serialize_common_long (version, (dcid, scid))) in
+        let consumed2 = Seq.length (serialize serialize_common_long (version, (dcid, scid))) in
         assert (parse parse_common_long x1 == Some ((version, (dcid, scid)), consumed2));
-        let x2 = S.slice x1 consumed2 (S.length x1) in
-        assert (x2 `S.equal` serialize (serialize_payload_length_pn last packet_number_length) (plpnl, packet_number));
-        let x3 = S.slice x2 0 (S.length x2) in
-        assert (x3 `S.equal` x2);
+        let x2 = Seq.slice x1 consumed2 (Seq.length x1) in
+        assert (x2 `Seq.equal` serialize (serialize_payload_length_pn last packet_number_length) (plpnl, packet_number));
+        let x3 = Seq.slice x2 0 (Seq.length x2) in
+        assert (x3 `Seq.equal` x2);
         serialize_nondep_then_eq (serialize_varint `serialize_filter` payload_and_pn_length_prop packet_number_length) (serialize_packet_number last packet_number_length) (plpnl, packet_number);
         assert (serialize (serialize_varint `serialize_filter` payload_and_pn_length_prop packet_number_length) plpnl == serialize serialize_varint plpnl);
         parse_serialize serialize_varint plpnl;
         parse_strong_prefix parse_varint (serialize serialize_varint plpnl) x3;
-        let consumed4 = S.length (serialize (serialize_varint `serialize_filter` payload_and_pn_length_prop packet_number_length) plpnl) in
-        assert (consumed4 == S.length (serialize serialize_varint plpnl));
+        let consumed4 = Seq.length (serialize (serialize_varint `serialize_filter` payload_and_pn_length_prop packet_number_length) plpnl) in
+        assert (consumed4 == Seq.length (serialize serialize_varint plpnl));
         assert (parse parse_varint x3 == Some (plpnl, consumed4));
         assert (putative_pn_offset cid_len x = Some (1 + consumed2 + consumed4));
         assert_norm (pn_offset' short_dcid_len last (MLong version dcid scid (MHandshake payload_length packet_number_length packet_number)) == 1 + consumed2 + 0 + consumed4)
@@ -1266,18 +1607,18 @@ let putative_pn_offset_correct h cid_len =
         serialize_nondep_then_eq serialize_common_long (serialize_payload_length_pn last packet_number_length) ((version, (dcid, scid)), (plpnl, packet_number));
         parse_serialize serialize_common_long (version, (dcid, scid));
         parse_strong_prefix parse_common_long (serialize serialize_common_long (version, (dcid, scid))) x1;
-        let consumed2 = S.length (serialize serialize_common_long (version, (dcid, scid))) in
+        let consumed2 = Seq.length (serialize serialize_common_long (version, (dcid, scid))) in
         assert (parse parse_common_long x1 == Some ((version, (dcid, scid)), consumed2));
-        let x2 = S.slice x1 consumed2 (S.length x1) in
-        assert (x2 `S.equal` serialize (serialize_payload_length_pn last packet_number_length) (plpnl, packet_number));
-        let x3 = S.slice x2 0 (S.length x2) in
-        assert (x3 `S.equal` x2);
+        let x2 = Seq.slice x1 consumed2 (Seq.length x1) in
+        assert (x2 `Seq.equal` serialize (serialize_payload_length_pn last packet_number_length) (plpnl, packet_number));
+        let x3 = Seq.slice x2 0 (Seq.length x2) in
+        assert (x3 `Seq.equal` x2);
         serialize_nondep_then_eq (serialize_varint `serialize_filter` payload_and_pn_length_prop packet_number_length) (serialize_packet_number last packet_number_length) (plpnl, packet_number);
         assert (serialize (serialize_varint `serialize_filter` payload_and_pn_length_prop packet_number_length) plpnl == serialize serialize_varint plpnl);
         parse_serialize serialize_varint plpnl;
         parse_strong_prefix parse_varint (serialize serialize_varint plpnl) x3;
-        let consumed4 = S.length (serialize (serialize_varint `serialize_filter` payload_and_pn_length_prop packet_number_length) plpnl) in
-        assert (consumed4 == S.length (serialize serialize_varint plpnl));
+        let consumed4 = Seq.length (serialize (serialize_varint `serialize_filter` payload_and_pn_length_prop packet_number_length) plpnl) in
+        assert (consumed4 == Seq.length (serialize serialize_varint plpnl));
         assert (parse parse_varint x3 == Some (plpnl, consumed4));
         assert (putative_pn_offset cid_len x = Some (1 + consumed2 + consumed4));
         assert_norm (pn_offset' short_dcid_len last (MLong version dcid scid (MZeroRTT payload_length packet_number_length packet_number)) == 1 + consumed2 + 0 + consumed4)
@@ -1303,8 +1644,8 @@ let lemma_header_parsing_correct
   parse_serialize (serialize_header cid_len32 (U64.uint_to_t last)) h;
   assert_norm ((parse_header_kind' cid_len32 (U64.uint_to_t last)).parser_kind_subkind == Some ParserStrong);
   parse_strong_prefix (lp_parse_header cid_len32 (U64.uint_to_t last)) s (s `Seq.append` c);
-  S.lemma_split (s `S.append` c) (S.length s);
-  assert (s `S.equal` S.slice s 0 (S.length s));
+  Seq.lemma_split (s `Seq.append` c) (Seq.length s);
+  assert (s `Seq.equal` Seq.slice s 0 (Seq.length s));
   match parse_header cid_len last Seq.(format_header h @| c) with
   | H_Failure -> ()
   | H_Success h' c' -> assert (h == h'); assert (c `Seq.equal` c')
@@ -1342,11 +1683,11 @@ let header_len'
     7 + FB.length dcid + FB.length scid +
     begin match spec with
     | MInitial token payload_length packet_number_length pn ->
-      S.length (serialize (serialize_bounded_varint 0 token_max_len) (FB.len token)) + FB.length token + S.length (serialize serialize_varint (payload_length `U64.add` Cast.uint32_to_uint64 packet_number_length)) + U32.v packet_number_length
+      Seq.length (serialize (serialize_bounded_varint 0 token_max_len) (FB.len token)) + FB.length token + Seq.length (serialize serialize_varint (payload_length `U64.add` Cast.uint32_to_uint64 packet_number_length)) + U32.v packet_number_length
     | MZeroRTT payload_length packet_number_length pn ->
-      S.length (serialize serialize_varint (payload_length `U64.add` Cast.uint32_to_uint64 packet_number_length)) + U32.v packet_number_length
+      Seq.length (serialize serialize_varint (payload_length `U64.add` Cast.uint32_to_uint64 packet_number_length)) + U32.v packet_number_length
     | MHandshake payload_length packet_number_length pn ->
-      S.length (serialize serialize_varint (payload_length `U64.add` Cast.uint32_to_uint64 packet_number_length)) + U32.v packet_number_length
+      Seq.length (serialize serialize_varint (payload_length `U64.add` Cast.uint32_to_uint64 packet_number_length)) + U32.v packet_number_length
     | MRetry unused odcid ->
       1 + FB.length odcid
     end
@@ -1391,7 +1732,7 @@ let header_len'_correct'_short
   ))
   (ensures (
     let h = MShort spin key_phase dcid packet_number_length packet_number in
-    header_len' h == S.length (serialize (serialize_header short_dcid_len last) h)
+    header_len' h == Seq.length (serialize (serialize_header short_dcid_len last) h)
   ))
 = 
   let h = MShort spin key_phase dcid packet_number_length packet_number in
@@ -1424,7 +1765,7 @@ let header_len'_correct'_long_initial
   ))
   (ensures (
     let h = MLong version dcid scid (MInitial token payload_length packet_number_length packet_number) in
-    header_len' h == S.length (serialize (serialize_header short_dcid_len last) h)
+    header_len' h == Seq.length (serialize (serialize_header short_dcid_len last) h)
   ))
 =
   let h = MLong version dcid scid (MInitial token payload_length packet_number_length packet_number) in
@@ -1459,7 +1800,7 @@ let header_len'_correct'_long_handshake
   ))
   (ensures (
     let h = MLong version dcid scid (MHandshake payload_length packet_number_length packet_number) in
-    header_len' h == S.length (serialize (serialize_header short_dcid_len last) h)
+    header_len' h == Seq.length (serialize (serialize_header short_dcid_len last) h)
   ))
 =
   let h = MLong version dcid scid (MHandshake payload_length packet_number_length packet_number) in
@@ -1492,7 +1833,7 @@ let header_len'_correct'_long_zeroRTT
   ))
   (ensures (
     let h = MLong version dcid scid (MZeroRTT payload_length packet_number_length packet_number) in
-    header_len' h == S.length (serialize (serialize_header short_dcid_len last) h)
+    header_len' h == Seq.length (serialize (serialize_header short_dcid_len last) h)
   ))
 =
   let h = MLong version dcid scid (MZeroRTT payload_length packet_number_length packet_number) in
@@ -1524,7 +1865,7 @@ let header_len'_correct'_long_retry
   ))
   (ensures (
     let h = MLong version dcid scid (MRetry unused odcid) in
-    header_len' h == S.length (serialize (serialize_header short_dcid_len last) h)
+    header_len' h == Seq.length (serialize (serialize_header short_dcid_len last) h)
   ))
 =
   let h = MLong version dcid scid (MRetry unused odcid) in
@@ -1544,7 +1885,7 @@ let header_len'_correct'
   (last: last_packet_number_t)
   (h: header' short_dcid_len last)
 : Lemma
-  (header_len' h == S.length (serialize (serialize_header short_dcid_len last) h))
+  (header_len' h == Seq.length (serialize (serialize_header short_dcid_len last) h))
 = match h with
   | MShort spin key_phase dcid packet_number_length packet_number ->
     header_len'_correct'_short short_dcid_len last spin key_phase dcid packet_number_length packet_number
