src/QUIC.Spec.Header.fsti
@@ -1,12 +1,71 @@
 module QUIC.Spec.Header
 include QUIC.Spec.Header.Base
 
+module Seq = FStar.Seq
+module HD = Spec.Hash.Definitions
+module AEAD = Spec.Agile.AEAD
+module U32 = FStar.UInt32
+module U64 = FStar.UInt64
+module PN = QUIC.Spec.PacketNumber.Base
+module Secret = QUIC.Secret.Int
+module AEAD = Spec.Agile.AEAD
+module Cipher = Spec.Agile.Cipher
+
+type cbytes' (is_retry: bool) = b: bytes { let l = Seq.length b in if is_retry then l == 0 else (19 <= l /\ l < max_cipher_length) }
+
+// Header serialization and protection
+
+val header_encrypt:
+  a:ea ->
+  hpk: Cipher.key (AEAD.cipher_alg_of_supported_alg a) ->
+  h: header ->
+  c: cbytes' (is_retry h) ->
+  GTot packet
+
+noeq
+type h_result =
+| H_Success:
+  h: header ->
+  cipher: cbytes' (is_retry h) ->
+  rem: bytes ->
+  h_result
+| H_Failure
+
+// Header protection removal and parsing
+
+val header_decrypt:
+  a:ea ->
+  hpk: Cipher.key (AEAD.cipher_alg_of_supported_alg a) ->
+  cid_len: nat { cid_len <= 20 } ->
+  last: nat { last + 1 < pow2 62 } ->
+  p: packet ->
+  GTot (r: h_result { match r with
+  | H_Failure -> True
+  | H_Success h c rem ->
+    is_valid_header h cid_len last /\
+    Seq.length rem <= Seq.length p /\
+    rem `Seq.equal` Seq.slice p (Seq.length p - Seq.length rem) (Seq.length p)
+  })
+
+// This is just functional correctness, but does not guarantee security:
+// decryption can succeed on an input that is not the encryption
+// of the same arguments (see QUIC.Spec.Old.*_malleable)
+val lemma_header_encryption_correct:
+  a:ea ->
+  k: Cipher.key (AEAD.cipher_alg_of_supported_alg a) ->
+  h:header ->
+  cid_len: nat { cid_len <= 20 /\ (MShort? h ==> cid_len == dcid_len h) } ->
+  last: nat { last + 1 < pow2 62 /\ ((~ (is_retry h)) ==> PN.in_window (Secret.v (pn_length h) - 1) last (Secret.v (packet_number h))) } ->
+  c: cbytes' (is_retry h) { has_payload_length h ==> Secret.v (payload_length h) == Seq.length c } ->
+  Lemma (
+    header_decrypt a k cid_len last (header_encrypt a k h c)
+    == H_Success h c Seq.empty)
+
+
 (*
 module Secret = QUIC.Secret.Int
 module U32 = FStar.UInt32
 module PN = QUIC.Spec.PacketNumber.Base
-module AEAD = Spec.Agile.AEAD
-module Cipher = Spec.Agile.Cipher
 
 noeq
 type h_result =
@@ -121,17 +180,17 @@ val format_header: h:header -> GTot (lbytes (header_len h))
 module BF = LowParse.BitFields
 
 val format_header_is_short: h: header -> Lemma
-  (MShort? h <==> BF.get_bitfield (U8.v (S.index (format_header h) 0)) 7 8 == 0)
+  (MShort? h <==> BF.get_bitfield (U8.v (Seq.index (format_header h) 0)) 7 8 == 0)
 
 val format_header_is_retry: h: header -> Lemma
   (is_retry h <==> (
-    BF.get_bitfield (U8.v (S.index (format_header h) 0)) 7 8 == 1 /\
-    BF.get_bitfield (U8.v (S.index (format_header h) 0)) 4 6 == 3
+    BF.get_bitfield (U8.v (Seq.index (format_header h) 0)) 7 8 == 1 /\
+    BF.get_bitfield (U8.v (Seq.index (format_header h) 0)) 4 6 == 3
   ))
 
 val format_header_pn_length: h: header -> Lemma
   (requires (~ (is_retry h)))
-  (ensures (BF.get_bitfield (U8.v (S.index (format_header h) 0)) 0 2 == U32.v (pn_length h) - 1))
+  (ensures (BF.get_bitfield (U8.v (Seq.index (format_header h) 0)) 0 2 == U32.v (pn_length h) - 1))
 
 val pn_offset: (h: header { ~ (is_retry h) }) -> GTot (n: nat { 0 < n /\ n + U32.v (pn_length h) == header_len h }) // need to know that packet number is the last field of the format
 
@@ -191,7 +250,7 @@ val lemma_header_parsing_correct:
     is_valid_header h cid_len last
   ))
   (ensures (
-    parse_header cid_len last S.(format_header h @| c)
+    parse_header cid_len last Seq.(format_header h @| c)
     == H_Success h c))
 
 // N.B. this is only true for a given DCID len
@@ -221,7 +280,7 @@ let lemma_header_parsing_post
   | H_Failure -> ()
   | H_Success h c ->
     lemma_header_parsing_correct h c cid_len last ;
-    lemma_header_parsing_safe cid_len last b (format_header h `S.append` c);
+    lemma_header_parsing_safe cid_len last b (format_header h `Seq.append` c);
     assert (b `Seq.equal` (format_header h `Seq.append` c));
     assert (Seq.slice b 0 (header_len h) `Seq.equal` format_header h);
     assert (c `Seq.equal` Seq.slice b (header_len h) (Seq.length b))
